Phi_System/IDE_CP_Reasoning2.thy
@@ -133,7 +133,7 @@ lemma [\<phi>reason 1215 for \<open>_ \<heavy_comma> _ \<Ztypecolon> \<v>\<a>\<l
   unfolding REMAINS_def Transformation_def by simp
 
 lemma [\<phi>reason 1210 for \<open>_ \<heavy_comma> _ \<Ztypecolon> \<v>\<a>\<l>[_] _ \<t>\<r>\<a>\<n>\<s>\<f>\<o>\<r>\<m>\<s> _ \<Ztypecolon> \<v>\<a>\<l>[_] _ \<r>\<e>\<m>\<a>\<i>\<n>\<s>[_] _ \<w>\<i>\<t>\<h> _\<close>
-                    if \<open>PLPR_Env.boolean_flag \<^const_name>\<open>ToA_flag_deep\<close> true o fst\<close>]:
+                    if \<open>PLPR_Env.boolean_flag \<^const_name>\<open>ToA_flag_deep\<close> true o Context.Proof o fst\<close>]:
   " y \<Ztypecolon> U \<t>\<r>\<a>\<n>\<s>\<f>\<o>\<r>\<m>\<s> x \<Ztypecolon> T \<w>\<i>\<t>\<h> P
 \<Longrightarrow> R \<heavy_comma> y \<Ztypecolon> \<v>\<a>\<l>[v] U \<t>\<r>\<a>\<n>\<s>\<f>\<o>\<r>\<m>\<s> x \<Ztypecolon> \<v>\<a>\<l>[v] T \<r>\<e>\<m>\<a>\<i>\<n>\<s>[True] R \<w>\<i>\<t>\<h> P"
   unfolding Transformation_def
